src/onerule.lean
@@ -10,6 +10,7 @@ def transforms (rule : production_rule) (oldWord newWord : string) : Prop :=
 ∃ v w : string, v ++ rule.input ++ w = oldWord ∧ v ++ rule.output ++ w = newWord
 
 
+
 -- Demonstrations
 
 def a_bb := production_rule.mk "a" "bb"
@@ -51,8 +52,8 @@ begin
   unfold transforms at assum,
   --rw a_bb at assum,
   have lit_in : a_bb.input = "a", refl,
-  have lit_out : a_bb.output = "bb", refl,
   rw lit_in at assum,
+  have lit_out : a_bb.output = "bb", refl,
   rw lit_out at assum,
   cases assum with v assum_,
   cases assum_ with w assum__,
@@ -64,10 +65,7 @@ begin
   have right_side : w = "ck",
   {
     rw left_side at hyp_before,
-    have foo: "l" ++ "a" = "la", refl,
-    rw foo at hyp_before,
-    have bar: "lack" = "la" ++ "ck", refl,
-    rw bar at hyp_before,
+    change "la" ++ w = "la" ++ "ck" at hyp_before,
     sorry,
     --exact list.append_inj_right hyp_before id,
   },
@@ -77,3 +75,7 @@ begin
   rw concaten at hyp_after,
   finish,
 end
+
+
+def asdf : list char := ['h', 'e', 'l', 'l', 'o']
+#print asdf
